isabelle/core/CoreFreeVars.thy
@@ -1,0 +1,34 @@
+theory CoreFreeVars
+  imports CoreSyntax
+begin
+
+(* Free variables of a core term *)
+fun core_term_free_vars :: "CoreTerm \<Rightarrow> string set" where
+  "core_term_free_vars (CoreTm_LitBool _) = {}"
+| "core_term_free_vars (CoreTm_LitInt _) = {}"
+| "core_term_free_vars (CoreTm_LitArray tms) = \<Union>(set (map core_term_free_vars tms))"
+| "core_term_free_vars (CoreTm_Var name) = {name}"
+| "core_term_free_vars (CoreTm_Cast _ tm) = core_term_free_vars tm"
+| "core_term_free_vars (CoreTm_Unop _ tm) = core_term_free_vars tm"
+| "core_term_free_vars (CoreTm_Binop _ lhs rhs) =
+    core_term_free_vars lhs \<union> core_term_free_vars rhs"
+| "core_term_free_vars (CoreTm_Let var rhs body) =
+    core_term_free_vars rhs \<union> (core_term_free_vars body - {var})"
+| "core_term_free_vars (CoreTm_Quantifier _ var _ body) =
+    core_term_free_vars body - {var}"
+| "core_term_free_vars (CoreTm_FunctionCall _ _ tmArgs) =
+    \<Union>(set (map core_term_free_vars tmArgs))"
+| "core_term_free_vars (CoreTm_VariantCtor _ _ payload) = core_term_free_vars payload"
+| "core_term_free_vars (CoreTm_Record flds) =
+    \<Union>(set (map (core_term_free_vars \<circ> snd) flds))"
+| "core_term_free_vars (CoreTm_RecordProj tm _) = core_term_free_vars tm"
+| "core_term_free_vars (CoreTm_VariantProj tm _) = core_term_free_vars tm"
+| "core_term_free_vars (CoreTm_ArrayProj arr idxs) =
+    core_term_free_vars arr \<union> \<Union>(set (map core_term_free_vars idxs))"
+| "core_term_free_vars (CoreTm_Match scrut arms) =
+    core_term_free_vars scrut \<union> \<Union>(set (map (core_term_free_vars \<circ> snd) arms))"
+| "core_term_free_vars (CoreTm_Sizeof tm) = core_term_free_vars tm"
+| "core_term_free_vars (CoreTm_Allocated tm) = core_term_free_vars tm"
+| "core_term_free_vars (CoreTm_Old tm) = core_term_free_vars tm"
+
+end
