isabelle/util/NatToString.thy
@@ -1,4 +1,4 @@
-theory NatToString 
+theory NatToString
   imports Main
 begin
 
@@ -10,5 +10,89 @@ fun nat_to_string :: "nat \<Rightarrow> string" where
 (* Generate synthetic field names "0", "1", "2", ... for tuple types *)
 definition tuple_field_names :: "nat \<Rightarrow> string list" where
   "tuple_field_names n = map nat_to_string [0..<n]"
+
+
+(* nat_to_string always produces a non-empty string *)
+lemma nat_to_string_nonempty: "nat_to_string n \<noteq> []"
+  by (induction n rule: nat_to_string.induct) auto
+
+(* The last character of nat_to_string encodes n mod 10 *)
+lemma nat_to_string_last: "last (nat_to_string n) = char_of (48 + n mod 10)"
+proof (induction n rule: nat_to_string.induct)
+  case (1 n)
+  show ?case
+  proof (cases "n < 10")
+    case True
+    hence "n mod 10 = n" by simp
+    thus ?thesis using True by simp
+  next
+    case False
+    thus ?thesis using nat_to_string_nonempty by simp
+  qed
+qed
+
+(* The butlast of nat_to_string for n >= 10 is nat_to_string (n div 10) *)
+lemma nat_to_string_butlast:
+  assumes "\<not> n < 10"
+  shows "butlast (nat_to_string n) = nat_to_string (n div 10)"
+  using assms nat_to_string_nonempty by (simp add: butlast_append)
+
+(* char_of is injective on the range 0..9 offset by 48 *)
+lemma char_of_digit_injective:
+  assumes "a < 10" "b < 10" "char_of (48 + a) = char_of (48 + (b::nat))"
+  shows "a = b"
+  using assms by auto
+
+(* nat_to_string is injective *)
+lemma nat_to_string_injective: "nat_to_string m = nat_to_string n \<Longrightarrow> m = n"
+proof (induction m arbitrary: n rule: less_induct)
+  case (less m)
+  show ?case
+  proof (cases "m < 10")
+    case m_small: True
+    show ?thesis
+    proof (cases "n < 10")
+      case True
+      from less.prems m_small True have "char_of (48 + m) = char_of (48 + n)"
+        by simp
+      thus ?thesis using char_of_digit_injective m_small True by blast
+    next
+      case False
+      \<comment> \<open>m < 10 gives length 1, n >= 10 gives length >= 2 - contradiction\<close>
+      from m_small have "length (nat_to_string m) = 1" by simp
+      moreover from False nat_to_string_nonempty
+      have "length (nat_to_string n) \<ge> 2"
+        by simp
+      ultimately show ?thesis using less.prems by simp
+    qed
+  next
+    case m_big: False
+    show ?thesis
+    proof (cases "n < 10")
+      case True
+      from True have "length (nat_to_string n) = 1" by simp
+      moreover from m_big nat_to_string_nonempty
+      have "length (nat_to_string m) \<ge> 2"
+        by simp
+      ultimately show ?thesis using less.prems by simp
+    next
+      case n_big: False
+      \<comment> \<open>Both >= 10: last characters match, so m mod 10 = n mod 10;
+         butlast matches, so nat_to_string (m div 10) = nat_to_string (n div 10),
+         and by IH, m div 10 = n div 10. Together: m = n.\<close>
+      from less.prems have last_eq: "last (nat_to_string m) = last (nat_to_string n)" by simp
+      hence mod_eq: "m mod 10 = n mod 10"
+        using nat_to_string_last char_of_digit_injective[of "m mod 10" "n mod 10"]
+        by simp
+      from less.prems have "butlast (nat_to_string m) = butlast (nat_to_string n)" by simp
+      hence "nat_to_string (m div 10) = nat_to_string (n div 10)"
+        using nat_to_string_butlast m_big n_big by simp
+      hence "m div 10 = n div 10"
+        using less.IH m_big by simp
+      thus ?thesis using mod_eq by (metis div_mod_decomp)
+    qed
+  qed
+qed
+
 
 end
